Assertion Logic + syntactic sugar
git-svn-id: orca@112

WP1-Programming-Languages-Semantics/WP11-C-semantics/src/IMP-Lenses/Hoare.thy
@@ -50,218 +50,213 @@ text {*A Hoare triple is represented by a pre-condition @{text P} a post-conditi
        and a program @{text C}. It says whenever the pre-condition @{text P} holds then the post-condition
        @{text Q} must hold after the execution of the program @{text C}.*}
 
-definition hoare :: "(bool ,  '\<alpha>) expr \<Rightarrow> '\<alpha> states \<Rightarrow> (bool ,  '\<alpha>) expr \<Rightarrow>  bool" ("\<lbrace>(1_)\<rbrace>/ (_)/\<lbrace>(1_)\<rbrace>") where
-"\<lbrace>P\<rbrace>C\<lbrace>Q\<rbrace> = ((bop implies P (C \<dagger> Q)) = \<guillemotleft>True\<guillemotright>)"
+abbreviation hoare :: "(bool ,  '\<alpha>) expr \<Rightarrow> '\<alpha> states \<Rightarrow> (bool ,  '\<alpha>) expr \<Rightarrow>  bool" ("\<lbrace>(1_)\<rbrace>/ (_)/\<lbrace>(1_)\<rbrace>") where
+"\<lbrace>P\<rbrace>C\<lbrace>Q\<rbrace> \<equiv> \<lceil>P \<longrightarrow>\<^sub>e (C \<dagger> Q)\<rceil>"
 
 lift_definition hoare_valid :: "(bool ,  '\<alpha>) expr \<Rightarrow> '\<alpha> states \<Rightarrow> (bool ,  '\<alpha>) expr \<Rightarrow> bool" ("\<Turnstile> {(1_)}/ (_)/ {(1_)}" 50) is
 "\<lambda>P C Q. (\<forall> \<sigma> \<sigma>'. P \<sigma> \<and> C \<sigma> = \<sigma>' \<longrightarrow> Q \<sigma>')" .
 
 lemma Hoare_eq:"\<Turnstile> {P}C{Q} = \<lbrace>P\<rbrace>C\<lbrace>Q\<rbrace>"
-    unfolding hoare_def  
-    by transfer (auto, meson)
+  by simp (transfer, auto)
 
-lemma Hoare_True [hoare]: "\<lbrace>P\<rbrace>C\<lbrace>\<guillemotleft>True\<guillemotright>\<rbrace>"
-  unfolding hoare_def 
-  by transfer auto
+lemma Hoare_True [hoare]: "\<lbrace>P\<rbrace>C\<lbrace>TRUE\<rbrace>"
+  by simp (transfer, auto)
 
-lemma Hoare_False [hoare]: "\<lbrace>\<guillemotleft>False\<guillemotright>\<rbrace>C\<lbrace>Q\<rbrace>"
-  unfolding hoare_def 
-  by transfer auto
+lemma Hoare_False [hoare]: "\<lbrace>FALSE\<rbrace>C\<lbrace>Q\<rbrace>"
+  by simp (transfer, auto)
 
 section {*Hoare for SKIP*}
 
 lemma Hoare_SKIP [hoare]: "\<lbrace>P\<rbrace>SKIP\<lbrace>P\<rbrace>"
-  unfolding hoare_def
-  by transfer auto
+   by simp (transfer, auto)
 
 section {*Hoare for assignment*}
 
-lemma Hoare_ASN:
- "\<lbrace>[X \<mapsto>\<^sub>s exp] \<dagger> P\<rbrace>X:== exp\<lbrace>P\<rbrace>" 
-   unfolding subst_upd_var_def hoare_def 
-  by transfer auto
+lemma Hoare_ASN: "\<lbrace>[X \<mapsto>\<^sub>s exp] \<dagger> P\<rbrace>X:== exp\<lbrace>P\<rbrace>" 
+  unfolding subst_upd_var_def 
+  by simp (transfer, auto)
 
 lemma  Hoare_ASN_bop_test:
   assumes 1:"weak_lens Y"  
   shows "\<lbrace>bop (op =) (VAR X) \<guillemotleft>1\<guillemotright>\<rbrace>
           Y:== (VAR X)
          \<lbrace>bop (op =) (VAR Y) \<guillemotleft>1\<guillemotright>\<rbrace>"
-  using 1 unfolding subst_upd_var_def hoare_def 
-  by transfer auto 
+  using 1 unfolding subst_upd_var_def 
+  by simp (transfer, auto) 
 
 lemma Hoare_ASN_uop1:
   assumes 1:"weak_lens X"  
   shows "\<lbrace>uop P exp\<rbrace>
           X:== exp
          \<lbrace>uop P (VAR X)\<rbrace>" 
-  using 1 unfolding subst_upd_var_def hoare_def   
-  by transfer auto
+  using 1 unfolding subst_upd_var_def    
+  by simp (transfer, auto) 
 
 lemma Hoare_ASN_uop2:
-  assumes 1:"weak_lens X"  and 2:"X \<sharp> exp"
+  assumes 1:"weak_lens X" and 2:"X \<sharp> exp"
   shows "\<lbrace>uop P exp\<rbrace>
           X:== exp
          \<lbrace>uop P exp\<rbrace>" 
-  using 1 2 unfolding subst_upd_var_def hoare_def unrest_def
-  by transfer auto
+  using 1 2 unfolding subst_upd_var_def unrest_def
+  by simp (transfer, auto) 
 
 lemma Hoare_ASN_uop3:
   assumes 1:"weak_lens X"
   shows "\<lbrace>uop P \<guillemotleft>exp\<guillemotright>\<rbrace>
           X:== \<guillemotleft>exp\<guillemotright>
          \<lbrace>uop P \<guillemotleft>exp\<guillemotright>\<rbrace>" 
-  using 1 unfolding subst_upd_var_def hoare_def unrest_def
-  by transfer auto
+  using 1 unfolding subst_upd_var_def unrest_def
+  by simp (transfer, auto) 
 
 lemma Hoare_Const_test:
   assumes 1:"weak_lens X" and 2:"X \<bowtie> Y"
-  shows "\<lbrace>bop (op =) (VAR Y) \<guillemotleft>2\<guillemotright>\<rbrace>X:== \<guillemotleft>2::int\<guillemotright>\<lbrace>bop (op =) (VAR Y) (VAR X)\<rbrace>" 
-  using 1 2 unfolding hoare_def subst_upd_var_def lens_indep_def
-  by transfer auto
+  shows "\<lbrace>(VAR Y) =\<^sub>e \<guillemotleft>2\<guillemotright>\<rbrace>X:== \<guillemotleft>2::int\<guillemotright>\<lbrace>(VAR Y) =\<^sub>e(VAR X)\<rbrace>" 
+  using 1 2 unfolding subst_upd_var_def lens_indep_def
+  by simp (transfer, auto)
 
 lemma Hoare_ASN_bop1:
   assumes 1:"weak_lens X" and 2:"X \<sharp> exp2"
   shows "\<lbrace>bop P exp1 exp2\<rbrace>
           X:== exp1
          \<lbrace>bop P (VAR X) exp2\<rbrace>" 
-  using 1 2 unfolding subst_upd_var_def hoare_def unrest_def 
-  by transfer auto
+  using 1 2 unfolding subst_upd_var_def unrest_def 
+  by simp (transfer, auto)
 
 lemma Hoare_ASN_bop2:
   assumes 1:"weak_lens X" and 2:"X \<sharp> exp1"
   shows "\<lbrace>bop P exp1 exp2\<rbrace>
           X:== exp2
          \<lbrace>bop P exp1 (VAR X)\<rbrace>" 
-  using 1 2 unfolding subst_upd_var_def hoare_def unrest_def 
-  by transfer auto
+  using 1 2 unfolding subst_upd_var_def unrest_def 
+  by simp (transfer, auto)
 
 lemma Hoare_ASN_bop3:
   assumes 1:"weak_lens X" 
   shows "\<lbrace>bop P exp1 \<guillemotleft>exp2\<guillemotright>\<rbrace>
           X:== exp1
          \<lbrace>bop P (VAR X) \<guillemotleft>exp2\<guillemotright>\<rbrace>" 
-  using 1 unfolding subst_upd_var_def hoare_def  
-  by transfer auto
+  using 1 unfolding subst_upd_var_def   
+  by simp (transfer, auto)
 
 lemma Hoare_ASN_bop4:
   assumes 1:"weak_lens X" 
   shows "\<lbrace>bop P \<guillemotleft>exp1\<guillemotright> exp2\<rbrace>
           X:== exp2
          \<lbrace>bop P \<guillemotleft>exp1\<guillemotright> (VAR X)\<rbrace>" 
-  using 1 unfolding subst_upd_var_def hoare_def  
-  by transfer auto
+  using 1 unfolding subst_upd_var_def   
+  by simp (transfer, auto)
 
 lemma Hoare_ASN_bop5:
   assumes 1:"weak_lens X" and 2:"X \<bowtie> Y"
   shows "\<lbrace>bop P (VAR Y) exp2\<rbrace>
           X:== exp2
          \<lbrace>bop P (VAR Y) (VAR X)\<rbrace>" 
-  using 1 2 unfolding subst_upd_var_def hoare_def lens_indep_def 
-  by transfer auto
+  using 1 2 unfolding subst_upd_var_def lens_indep_def 
+  by simp (transfer, auto)
 
 lemma Hoare_ASN_trop1:
   assumes 1:"weak_lens X"  and 2:"X \<sharp> exp2" and 3:"X \<sharp> exp3"
   shows "\<lbrace>trop P exp1 exp2 exp3\<rbrace>
           X:== exp1
          \<lbrace>trop P (VAR X) exp2 exp3\<rbrace>" 
-  using 1 2 3 unfolding subst_upd_var_def hoare_def unrest_def 
-  by transfer auto
+  using 1 2 3 unfolding subst_upd_var_def unrest_def 
+  by simp (transfer, auto)
 
 lemma Hoare_ASN_trop2:
   assumes 1:"weak_lens X"  and 2:"X \<sharp> exp1" and 3:"X \<sharp> exp3"
   shows "\<lbrace>trop P exp1 exp2 exp3\<rbrace>
           X:== exp2
          \<lbrace>trop P exp1 (VAR X) exp3\<rbrace>" 
-  using 1 2 3 unfolding subst_upd_var_def hoare_def unrest_def 
-  by transfer auto
+  using 1 2 3 unfolding subst_upd_var_def unrest_def 
+  by simp (transfer, auto)
 
 lemma Hoare_ASN_trop3:
   assumes 1:"weak_lens X" and 2:"X \<sharp> exp1" and 3:"X \<sharp> exp2"
   shows "\<lbrace>trop P exp1 exp2 exp3\<rbrace> 
           X:== exp3
          \<lbrace>trop P exp1 exp2 (VAR X)\<rbrace>" 
-  using 1 2 3 unfolding subst_upd_var_def hoare_def unrest_def 
-  by transfer auto
+  using 1 2 3 unfolding subst_upd_var_def unrest_def 
+  by simp (transfer, auto)
 
 lemma Hoare_ASN_trop4:
   assumes 1:"weak_lens X" 
   shows "\<lbrace>trop P exp1 \<guillemotleft>exp2\<guillemotright> \<guillemotleft>exp3\<guillemotright>\<rbrace>
           X:== exp1
          \<lbrace>trop P (VAR X) \<guillemotleft>exp2\<guillemotright> \<guillemotleft>exp3\<guillemotright>\<rbrace>" 
-  using 1  unfolding subst_upd_var_def hoare_def  
-  by transfer auto
+  using 1  unfolding subst_upd_var_def   
+  by simp (transfer, auto)
 
 lemma Hoare_ASN_trop5:
   assumes 1:"weak_lens X" 
   shows "\<lbrace>trop P \<guillemotleft>exp1\<guillemotright> exp2 \<guillemotleft>exp3\<guillemotright>\<rbrace>
           X:== exp2 
          \<lbrace>trop P \<guillemotleft>exp1\<guillemotright> (VAR X) \<guillemotleft>exp3\<guillemotright>\<rbrace>" 
-  using 1  unfolding subst_upd_var_def hoare_def  
-  by transfer auto
+  using 1  unfolding subst_upd_var_def   
+  by simp (transfer, auto)
 
 lemma Hoare_ASN_trop6:
   assumes 1:"weak_lens X" 
   shows "\<lbrace>trop P \<guillemotleft>exp1\<guillemotright> \<guillemotleft>exp2\<guillemotright> exp3\<rbrace>
           X:== exp3
          \<lbrace>trop P \<guillemotleft>exp1\<guillemotright> \<guillemotleft>exp2\<guillemotright> (VAR X)\<rbrace>" 
-  using 1  unfolding subst_upd_var_def hoare_def  
-  by transfer auto
+  using 1  unfolding subst_upd_var_def   
+  by simp (transfer, auto)
 
 lemma Hoare_ASN_qtop1:
   assumes 1:"weak_lens X"  and 2:"X \<sharp> exp2" and 3:"X \<sharp> exp3"  and 4:"X \<sharp> exp4"
   shows "\<lbrace>qtop P exp1 exp2 exp3 exp4\<rbrace>
           X:== exp1
          \<lbrace>qtop P (VAR X) exp2 exp3 exp4\<rbrace>" 
-  using 1 2 3 4unfolding subst_upd_var_def hoare_def unrest_def 
-  by transfer auto
+  using 1 2 3 4unfolding subst_upd_var_def unrest_def 
+  by simp (transfer, auto)
 
 lemma Hoare_ASN_qtop2:
   assumes 1:"weak_lens X" and 2:"X \<sharp> exp1" and 3:"X \<sharp> exp3" and 4:"X \<sharp> exp4"
   shows "\<lbrace>qtop P exp1 exp2 exp3 exp4\<rbrace>
           X:== exp2
          \<lbrace>qtop P exp1 (VAR X) exp3 exp4\<rbrace>" 
-  using 1 2 3 4 unfolding subst_upd_var_def hoare_def unrest_def 
-  by transfer auto
+  using 1 2 3 4 unfolding subst_upd_var_def unrest_def 
+  by simp (transfer, auto)
 
 lemma Hoare_ASN_qtop3:
   assumes 1:"weak_lens X" and 2:"X \<sharp> exp1" and 3:"X \<sharp> exp2" and 4:"X \<sharp> exp4"
   shows "\<lbrace>qtop P exp1 exp2 exp3 exp4\<rbrace>
           X:== exp3
          \<lbrace>qtop P exp1 exp2 (VAR X) exp4\<rbrace>" 
-  using 1 2 3 4 unfolding subst_upd_var_def hoare_def unrest_def 
-  by transfer auto
+  using 1 2 3 4 unfolding subst_upd_var_def unrest_def 
+  by simp (transfer, auto)
 
 lemma Hoare_ASN_qtop4:
   assumes 1:"weak_lens X" and 2:"X \<sharp> exp1" and 3:"X \<sharp> exp2" and 4:"X \<sharp> exp3"
   shows "\<lbrace>qtop P exp1 exp2 exp3 exp4\<rbrace>
           X:== exp4
          \<lbrace>qtop P exp1 exp2 exp3 (VAR X)\<rbrace>" 
-  using 1 2 3 4 unfolding subst_upd_var_def hoare_def unrest_def 
-  by transfer auto
+  using 1 2 3 4 unfolding subst_upd_var_def unrest_def 
+  by simp (transfer, auto)
 
 lemma Hoare_ASN_qtop5:
   assumes 1:"weak_lens X" 
   shows "\<lbrace>qtop P exp1 \<guillemotleft>exp2\<guillemotright> \<guillemotleft>exp3\<guillemotright> \<guillemotleft>exp4\<guillemotright>\<rbrace>
           X:== exp1
          \<lbrace>qtop P (VAR X) \<guillemotleft>exp2\<guillemotright> \<guillemotleft>exp3\<guillemotright> \<guillemotleft>exp4\<guillemotright>\<rbrace> " 
-  using 1 unfolding subst_upd_var_def hoare_def  
-  by transfer auto
+  using 1 unfolding subst_upd_var_def   
+  by simp (transfer, auto)
 
 lemma Hoare_ASN_qtop6:
   assumes 1:"weak_lens X" 
   shows "\<lbrace>qtop P \<guillemotleft>exp1\<guillemotright> exp2 \<guillemotleft>exp3\<guillemotright> \<guillemotleft>exp4\<guillemotright>\<rbrace>
           X:== exp2
          \<lbrace>qtop P \<guillemotleft>exp1\<guillemotright> (VAR X) \<guillemotleft>exp3\<guillemotright> \<guillemotleft>exp4\<guillemotright>\<rbrace>" 
-  using 1  unfolding subst_upd_var_def hoare_def  
-  by transfer auto
+  using 1  unfolding subst_upd_var_def   
+  by simp (transfer, auto)
 
 lemma Hoare_ASN_qtop7:
   assumes 1:"weak_lens X" 
   shows "\<lbrace>qtop P \<guillemotleft>exp1\<guillemotright> \<guillemotleft>exp2\<guillemotright> exp3 \<guillemotleft>exp4\<guillemotright>\<rbrace>
           X:== exp3
          \<lbrace>qtop P \<guillemotleft>exp1\<guillemotright> \<guillemotleft>exp2\<guillemotright> (VAR X) \<guillemotleft>exp4\<guillemotright>\<rbrace>" 
-  using 1  unfolding subst_upd_var_def hoare_def  
-  by transfer auto
+  using 1 unfolding subst_upd_var_def  
+  by simp (transfer, auto)
 
 section {*Hoare for Sequential Composition*}
 
@@ -269,33 +264,34 @@ lemma Hoare_SEQ:
   assumes 1:"\<lbrace>P\<rbrace>C1\<lbrace>Q\<rbrace>"  
   and     2:"\<lbrace>Q\<rbrace>C2\<lbrace>R\<rbrace>"
   shows "\<lbrace>P\<rbrace>C1;C2\<lbrace>R\<rbrace>" 
-  using 1 2 unfolding hoare_def   
-  by transfer (metis comp_apply)
+  using 1 2 
+  by simp (transfer, (metis comp_apply))
 
 section {*Hoare for Conditional*}
 
 lemma Hoare_COND:
-  assumes 1:"\<lbrace>bop conj P b\<rbrace>C1\<lbrace>Q\<rbrace>"  
-  and     2:"\<lbrace>bop conj P (uop Not b)\<rbrace>C2\<lbrace>Q\<rbrace>"
+  assumes 1:"\<lbrace>P \<and>\<^sub>e b\<rbrace>C1\<lbrace>Q\<rbrace>"  
+  and     2:"\<lbrace> P \<and>\<^sub>e (\<not>\<^sub>e b)\<rbrace>C2\<lbrace>Q\<rbrace>"
   shows "\<lbrace>P\<rbrace>IF b THEN C1 ELSE C2\<lbrace>Q\<rbrace>" 
-  using 1 2 unfolding hoare_def 
-  by transfer (metis (full_types, hide_lams))   
+  using 1 2 
+  by simp (transfer , metis (full_types, hide_lams))   
 
 section {*Hoare for Consequence*}
 
 lemma Hoare_CONSEQ:
-  assumes 1:"(bop implies P' P) = \<guillemotleft>True\<guillemotright>"  
-  and     2:"(bop implies Q Q') = \<guillemotleft>True\<guillemotright>"
+  assumes 1:"\<lceil>P' \<longrightarrow>\<^sub>e P\<rceil>"  
+  and     2:"\<lceil>Q \<longrightarrow>\<^sub>e Q'\<rceil>"
   shows "\<lbrace>P\<rbrace>C\<lbrace>Q\<rbrace> \<longrightarrow> \<lbrace>P'\<rbrace>C\<lbrace>Q'\<rbrace>" 
-  using 1 2 unfolding hoare_def
-  by transfer meson 
+  using 1 2
+  by simp (transfer, meson) 
 
 section {*Hoare for While-loop*}
 
 lemma Hoare_WHILE:
-  assumes 1:"\<lbrace>bop conj P b\<rbrace>C\<lbrace>P\<rbrace>"  
-  shows "\<lbrace>P\<rbrace>WHILE b DO C OD\<lbrace>bop conj P (uop Not b)\<rbrace>" 
-  using 1 unfolding hoare_def RelInv_def Rel_def W_def
+  assumes 1:"\<lbrace>P \<and>\<^sub>e b\<rbrace>C\<lbrace>P\<rbrace>"  
+  shows "\<lbrace>P\<rbrace>WHILE b DO C OD\<lbrace>P \<and>\<^sub>e (\<not>\<^sub>eb)\<rbrace>" 
+  using 1 unfolding RelInv_def Rel_def W_def
+  apply simp apply transfer
 oops  
 
 
