WP1-Programming-Languages-Semantics/WP11-C-semantics/src/IMP-Lenses/Expressions.thy
@@ -1,44 +1,122 @@
 
-section {*expressions*}
+section {*Expressions*}
+text{*In this section we introduce the type of variables and expressions used in our 
+      specification language. Since we use a shallow embedding for expressions we introduce
+      the different lifting operators between the different types.*}
 
 theory Expressions imports Lenses "~~/src/Tools/Adhoc_Overloading" 
 
 begin
-
+subsection {*Types*}
 text{*In this setting the state-space is represented by the 
       type @{text "\<alpha>"}, and expressions by the type @{text "\<tau>"}*}
+
 type_synonym ('\<tau> , '\<alpha> ) var = "('\<tau> \<Longrightarrow> '\<alpha>)"         
 type_synonym  ('\<tau> ,'\<alpha>) expr  =  "'\<alpha>  \<Rightarrow> '\<tau>" 
 
+subsection {*Lifting vars to to expressions*}
 
-
-  -- "arithmetic and boolean expressions are not modelled explicitly here,"
-
-text {*Lifting vars to expr*}
 lift_definition imp_var :: "('\<tau>, '\<alpha>) var \<Rightarrow> ('\<tau>, '\<alpha>) expr" ("VAR _") is 
   lens_get .
 
+subsection {*Lifting HOL functions to expressions*}
 
-text {*Lifting HOL constant functions to expr*}
 lift_definition Const :: "'t \<Rightarrow> ('t, '\<alpha>) expr" ("\<guillemotleft>_\<guillemotright>") is 
-  "\<lambda> v b. v" .
+  "\<lambda> v \<sigma>. v" .
 
-lift_definition uop :: "('a \<Rightarrow> 'b) \<Rightarrow> ('a, '\<alpha>) expr \<Rightarrow> ('b, '\<alpha>) expr"
-  is "\<lambda> f e b. f (e b)" .
+lift_definition uop :: "('a \<Rightarrow> 'b) \<Rightarrow> ('a, '\<alpha>) expr \<Rightarrow> ('b, '\<alpha>) expr" is 
+  "\<lambda> f e \<sigma>. f (e \<sigma>)" .
 
 lift_definition bop ::
-  "('a \<Rightarrow> 'b \<Rightarrow> 'c) \<Rightarrow> ('a, '\<alpha>) expr \<Rightarrow> ('b, '\<alpha>) expr \<Rightarrow> ('c, '\<alpha>) expr"
-  is "\<lambda> f u v b. f (u b) (v b)" .
+  "('a \<Rightarrow> 'b \<Rightarrow> 'c) \<Rightarrow> ('a, '\<alpha>) expr \<Rightarrow> ('b, '\<alpha>) expr \<Rightarrow> ('c, '\<alpha>) expr" is 
+  "\<lambda> f x y \<sigma>. f (x \<sigma>) (y \<sigma>)" .
 
 lift_definition trop ::
-  "('a \<Rightarrow> 'b \<Rightarrow> 'c \<Rightarrow> 'd) \<Rightarrow> ('a, '\<alpha>) expr \<Rightarrow> ('b, '\<alpha>) expr \<Rightarrow> ('c, '\<alpha>) expr \<Rightarrow> ('d, '\<alpha>) expr"
-  is "\<lambda> f u v w b. f (u b) (v b) (w b)" .
+  "('a \<Rightarrow> 'b \<Rightarrow> 'c \<Rightarrow> 'd) \<Rightarrow> ('a, '\<alpha>) expr \<Rightarrow> ('b, '\<alpha>) expr \<Rightarrow> ('c, '\<alpha>) expr \<Rightarrow> ('d, '\<alpha>) expr" is
+  "\<lambda> f x y z \<sigma>. f (x \<sigma>) (y \<sigma>) (z \<sigma>)" .
 
 lift_definition qtop ::
   "('a \<Rightarrow> 'b \<Rightarrow> 'c \<Rightarrow> 'd \<Rightarrow> 'e) \<Rightarrow> 
    ('a, '\<alpha>) expr \<Rightarrow> ('b, '\<alpha>) expr \<Rightarrow> ('c, '\<alpha>) expr \<Rightarrow> ('d, '\<alpha>) expr \<Rightarrow>
-   ('e, '\<alpha>) expr"
-  is "\<lambda> f u v w x b. f (u b) (v b) (w b) (x b)" .
+   ('e, '\<alpha>) expr" is
+   "\<lambda> f x y z w \<sigma>. f (x \<sigma>) (y \<sigma>) (z \<sigma>) (w \<sigma>)" .
+
+subsection {*Lifting HOL Constant operations to expressions*}
+
+definition True_expr :: "(bool, '\<alpha>) expr" ("TRUE")
+where [simp]:"True_expr = \<guillemotleft>True\<guillemotright>"
+
+definition False_expr :: "(bool, '\<alpha>) expr" ("FALSE")
+where [simp]:"False_expr = \<guillemotleft>False\<guillemotright>"
+
+subsection {*Lifting HOL unary operations to expressions*}
+
+definition uminus_expr :: "('a::uminus, '\<alpha>) expr \<Rightarrow> ('a, '\<alpha>) expr" ("-\<^sub>e _" [81] 80) 
+where [simp]:"uminus_expr x = uop uminus x"
+
+definition inverse_expr :: "('a::inverse, '\<alpha>) expr \<Rightarrow> ('a, '\<alpha>) expr"
+where [simp]:"inverse_expr x = uop inverse x"
+
+definition sgn_expr ::"('a::sgn, '\<alpha>) expr \<Rightarrow> ('a, '\<alpha>) expr" ("SGN")
+where [simp]:"sgn_expr x = uop sgn x"
+
+definition abs_expr ::"('a::abs, '\<alpha>) expr \<Rightarrow> ('a, '\<alpha>) expr" ("ABS")
+where [simp]:"abs_expr x = uop abs x"
+
+definition Not_expr :: "(bool, '\<alpha>) expr \<Rightarrow> (bool, '\<alpha>) expr"("\<not>\<^sub>e _" [40] 40)
+where [simp]:"Not_expr bexp = uop Not bexp "
+
+definition All_expr :: "('a \<Rightarrow> bool, '\<alpha>) expr \<Rightarrow> (bool, '\<alpha>) expr"(binder "\<forall>\<^sub>e" 10)
+where [simp]:"All_expr P = uop All P"
+
+definition Ex_expr :: "('a \<Rightarrow> bool, '\<alpha>) expr \<Rightarrow> (bool, '\<alpha>) expr"(binder "\<exists>\<^sub>e" 10)
+where [simp]:"Ex_expr P = uop Ex P"
+
+definition Ex1_expr :: "('a \<Rightarrow> bool, '\<alpha>) expr \<Rightarrow> (bool, '\<alpha>) expr"(binder "\<exists>!\<^sub>e" 10)
+where [simp]:"Ex1_expr P = uop Ex1 P"
+
+subsection {*Lifting HOL binary operations to expressions*}
+
+definition eq_expr :: "('a, '\<alpha>) expr \<Rightarrow> ('a, '\<alpha>) expr \<Rightarrow> (bool, '\<alpha>) expr" (infixl "=\<^sub>e" 50)
+where [simp]:"eq_expr x y = bop HOL.eq x y"
+
+definition conj_expr :: "(bool, '\<alpha>) expr \<Rightarrow> (bool, '\<alpha>) expr \<Rightarrow> (bool, '\<alpha>) expr"(infixr "\<and>\<^sub>e" 35)
+where [simp]:"conj_expr bexp1 bexp2 =  bop conj bexp1 bexp2"
+
+definition disj_expr :: "(bool, '\<alpha>) expr \<Rightarrow> (bool, '\<alpha>) expr \<Rightarrow> (bool, '\<alpha>) expr"(infixr "\<or>\<^sub>e" 30)
+where [simp]:"disj_expr bexp1 bexp2 =  bop disj bexp1 bexp2"
+
+definition implies_expr :: "(bool, '\<alpha>) expr \<Rightarrow> (bool, '\<alpha>) expr \<Rightarrow> (bool, '\<alpha>) expr"(infixr "\<longrightarrow>\<^sub>e" 25)
+where [simp]:"implies_expr bexp1 bexp2 =  bop implies bexp1 bexp2"
+
+definition plus_expr :: "('a::plus, '\<alpha>) expr \<Rightarrow> ('a, '\<alpha>) expr \<Rightarrow> ('a, '\<alpha>) expr" (infixl "+\<^sub>e" 65)
+where [simp]:"plus_expr x y = bop (op +) x y"
+
+definition minus_expr :: "('a::minus, '\<alpha>) expr \<Rightarrow> ('a, '\<alpha>) expr \<Rightarrow> ('a, '\<alpha>) expr" (infixl "-\<^sub>e" 65)
+where [simp]:"minus_expr x y = bop (op -) x y"
+
+definition times_expr :: "('a::times, '\<alpha>) expr \<Rightarrow> ('a, '\<alpha>) expr \<Rightarrow> ('a, '\<alpha>) expr" (infixl "*\<^sub>e" 65)
+where [simp]:"times_expr x y = bop (op *) x y"
+
+definition divide_expr :: "('a::divide, '\<alpha>) expr \<Rightarrow> ('a, '\<alpha>) expr \<Rightarrow> ('a, '\<alpha>) expr" (infixl "div\<^sub>e" 70)
+where [simp]: "divide_expr x y = bop divide x y"
+
+definition mod_expr ::"('a::Divides.div, '\<alpha>) expr \<Rightarrow> ('a, '\<alpha>) expr \<Rightarrow> ('a, '\<alpha>) expr" (infixl "mod\<^sub>e" 70)
+where [simp]:"mod_expr x y = bop (op mod) x y"
+
+definition less_eq_expr :: "('a::ord, '\<alpha>) expr \<Rightarrow> ('a, '\<alpha>) expr \<Rightarrow> (bool, '\<alpha>) expr" ("(_/ \<le>\<^sub>e _)"  [51, 51] 50)
+where  [simp]: "less_eq_expr x y =  bop (op \<le>) x y" 
+
+definition less_expr :: "('a::ord, '\<alpha>) expr \<Rightarrow> ('a, '\<alpha>) expr \<Rightarrow> (bool, '\<alpha>) expr"  ("(_/ <\<^sub>e _)"  [51, 51] 50)
+where [simp]:"less_expr x y = (bop less x y)"
+
+subsection {*Drop boolean expressions*}
+
+lemma drop_bexp_eq:"(P = TRUE) = (\<forall>\<sigma>. P \<sigma>)"
+  by (simp, transfer, auto)
+
+lift_definition drop_bexp :: "(bool ,  '\<alpha>) expr \<Rightarrow> bool" ("\<lceil>_\<rceil>")is
+"\<lambda>P. (\<forall>\<sigma>. P \<sigma>)".
 
 
 end
